fsub/autosubst2_dctx/prop_subtyping.v
@@ -7,7 +7,6 @@ Require Import fsub.autosubst2_dctx.prop_basic.
 From Coq Require Import ssreflect ssrfun ssrbool.
 From Hammer Require Import Tactics.
 Require Import Coq.Program.Equality.
-Require Import Nat.
 Require Import List.
 Require Import Arith.
 
@@ -44,7 +43,6 @@ Proof.
     hauto ctrs:lookup_tvar.
 Qed.
 
-
 Lemma lookup_tvar_rebounding : forall Δ1 Δ2 B,
   lookup_tvar (length Δ2) (Δ2 ++ B :: Δ1) (B ⟨fun X => 1 + (length Δ2 + X) ⟩) /\
   (forall X A B', X <> length Δ2 -> 
@@ -54,7 +52,7 @@ Proof.
   split. 
   - induction Δ2; simpl; asimpl; try hauto ctrs:lookup_tvar.
     + replace (ren_typ (fun X : nat => S (S (length Δ2 + X))) B) with
-      (B ⟨fun X : nat => 1 + (length Δ2 + X)⟩ ⟨ ↑⟩ ) by (asimpl; auto).
+      (B ⟨fun X : nat => 1 + (length Δ2 + X)⟩ ⟨↑⟩ ) by (asimpl; auto).
       hauto ctrs:lookup_tvar.
   - intros. dependent induction H0.
     + destruct Δ2; simpl in *; try hauto ctrs:lookup_tvar.
@@ -63,6 +61,14 @@ Qed.
 
 Lemma conj' (A B : Prop) : A -> (A -> B) -> A /\ B.
 Proof. tauto. Qed.
+
+Theorem subtyping_reflexivity Δ A :
+  Δ ⊢ A ->
+  Δ ⊢ A <: A.
+Proof.
+  move : Δ. induction A; intros; try hauto ctrs:subtyping.
+  - apply sub_top; auto.
+Qed.
 
 Theorem subtyping_transitivity_narrowing n:
   (forall Δ A B C,  
@@ -79,31 +85,31 @@ Proof.
   induction (lt_wf n) as [n _ IH].
   intros. apply conj'.
   - intros. move : C H1. induction H0; intros; try hauto ctrs:subtyping.
-      + inversion H1; subst.
-        * hauto ctrs:subtyping. 
-      + simpl in *. 
-        inversion H1; subst.
-        * eapply sub_top. hauto use:sub_wf_typ1, sub_wf_typ2.
-        * eapply sub_arrow.
-          --  edestruct (IH (typ_size B1)). hfcrush. hauto. 
-          --  edestruct (IH (typ_size B2)). hfcrush. hauto. 
-      + inversion H1; subst.
-        * eapply sub_top. simpl in *. split.
-          -- hauto use:sub_wf_typ1, sub_wf_typ2.
-          -- eapply wf_typ_renaming_tvar' with (ξ:=id) (A:=A2) (A':=A2) (Δ:=B1::Δ);
-            hauto unfold:ctx_tvar_rename_weak inv:lookup_tvar ctrs:lookup_tvar use:sub_wf_typ1, sub_wf_typ2 simp+:asimpl.
-        * eapply sub_all; eauto.
-          -- edestruct (IH (typ_size B1)). hfcrush. auto. hauto. 
-          -- edestruct (IH (typ_size B1)). eauto. hfcrush. eauto. 
-             edestruct (IH (typ_size B2)). hfcrush. eauto.
-             replace (B0 :: Δ) with (nil ++ B0 :: Δ) by auto.
-             eapply H2; eauto.
+    + inversion H1; subst.
+      * hauto ctrs:subtyping. 
+    + simpl in *. 
+      inversion H1; subst.
+      * eapply sub_top. hauto use:sub_wf_typ1, sub_wf_typ2.
+      * eapply sub_arrow.
+        -- edestruct (IH (typ_size B1)). hfcrush. hauto. 
+        -- edestruct (IH (typ_size B2)). hfcrush. hauto. 
+    + inversion H1; subst.
+      * eapply sub_top. simpl in *. split.
+        -- hauto use:sub_wf_typ1, sub_wf_typ2.
+        -- eapply wf_typ_renaming_tvar' with (ξ:=id) (A:=A2) (A':=A2) (Δ:=B1::Δ);
+          hauto unfold:ctx_tvar_rename_weak inv:lookup_tvar ctrs:lookup_tvar use:sub_wf_typ1, sub_wf_typ2 simp+:asimpl.
+      * eapply sub_all; eauto.
+        -- edestruct (IH (typ_size B1)). hfcrush. auto. hauto. 
+        -- edestruct (IH (typ_size B1)). eauto. hfcrush. eauto. 
+           edestruct (IH (typ_size B2)). hfcrush. eauto.
+           replace (B0 :: Δ) with (nil ++ B0 :: Δ) by auto.
+           eapply H2; eauto.
   - intros Htrans. intros. move : B' H1. dependent induction H0; intros; auto.
     + eapply sub_top.
       eapply wf_typ_renaming_tvar' with (ξ:=id); 
         hauto use:ctx_tvar_rename_weak_rebounding simp+:asimpl.
     + eapply sub_tvar_refl; eauto.
-       eapply wf_typ_renaming_tvar' with (ξ:=id) (A:=typ_var X); 
+      eapply wf_typ_renaming_tvar' with (ξ:=id) (A:=typ_var X); 
         hauto use:ctx_tvar_rename_weak_rebounding simp+:asimpl.
     + edestruct (Nat.eq_dec X (length Δ2)).
       * subst. 
@@ -125,7 +131,9 @@ Proof.
 Qed.
 
 Corollary subtyping_transitivity Δ A B C:
-  Δ ⊢ A <: B -> Δ ⊢ B <: C -> Δ ⊢ A <: C.
+  Δ ⊢ A <: B -> 
+  Δ ⊢ B <: C -> 
+  Δ ⊢ A <: C.
 Proof.
   eapply subtyping_transitivity_narrowing; eauto.
 Qed.
@@ -136,4 +144,31 @@ Corollary subtyping_narrowing Δ1 Δ2 A B B' C:
   Δ2 ++ B' :: Δ1 ⊢ A <: C.
 Proof.
   eapply subtyping_transitivity_narrowing; eauto.
+Qed.
+
+Definition ctx_tvar_subst Δ Δ' σ :=
+  forall X A, lookup_tvar X Δ A -> Δ' ⊢ σ X <: A [σ].
+
+Lemma subtyping_subst Δ Δ' A B σ :
+  Δ ⊢ A <: B ->
+  ctx_tvar_subst Δ Δ' σ ->
+  Δ' ⊢ A [ σ ] <: B [ σ ].
+Proof.
+  move => H. move : Δ' σ. elim: Δ A B / H; intros.
+  - asimpl.
+    hauto unfold:ctx_tvar_subst_wf,ctx_tvar_subst use:wf_typ_subst_tvar,sub_wf_typ1,sub_wf_typ2 ctrs:subtyping.
+  - hauto use:subtyping_reflexivity,sub_wf_typ1 unfold:ctx_tvar_subst ctrs:subtyping.
+  - hauto use:subtyping_transitivity unfold:ctx_tvar_subst ctrs:subtyping.
+  - apply sub_arrow; hauto.
+  - asimpl. apply sub_all; eauto.
+    + hauto unfold:ctx_tvar_subst_wf,ctx_tvar_subst use:wf_typ_subst_tvar,sub_wf_typ1,sub_wf_typ2 ctrs:subtyping.
+    + apply H0. unfold ctx_tvar_subst in *. intros.
+      inversion H2; subst; asimpl.
+      eapply sub_tvar_bound with (A:=B1 [σ] ⟨ ↑ ⟩). econstructor.
+      replace (subst_typ (σ >> (ren_typ ↑)) B1) with (B1 [σ] ⟨ ↑ ⟩) by (asimpl; auto).
+      eapply sub_weakening_tvar0. 
+      hauto unfold:ctx_tvar_subst_wf inv:lookup_tvar ctrs:lookup_tvar use:sub_wf_typ1,sub_wf_typ2,subtyping_reflexivity,wf_typ_subst_tvar.
+      replace (subst_typ (σ >> (ren_typ ↑)) A0) with (A0 [σ] ⟨ ↑ ⟩) by (asimpl; auto).
+      eapply sub_weakening_tvar0. 
+      hauto unfold:ctx_tvar_subst_wf inv:lookup_tvar ctrs:lookup_tvar use:sub_wf_typ1,sub_wf_typ2,subtyping_reflexivity,wf_typ_subst_tvar.
 Qed.
