fsub/autosubst2_dctx/prop_typing.v
@@ -1,0 +1,6 @@
+Require Import common.prop_as_core.
+Require Import common.prop_as_unscoped.
+Require Import fsub.autosubst2_dctx.def_as2.
+Require Import fsub.autosubst2_dctx.def_extra.
+Require Import fsub.autosubst2_dctx.prop_basic.
+Require Import fsub.autosubst2_dctx.prop_subtyping.
